prove correctness of apply and compose

TextOperation.v
@@ -3,6 +3,7 @@ Module TextOperation.
 Require Import
   Coq.Strings.Ascii
   Coq.Strings.String
+  Coq.Arith.Peano_dec
   Coq.Lists.List.
 
 Section TextOperation.
@@ -10,7 +11,7 @@ Section TextOperation.
 Variable A : Type.
 
 Local Notation "[ ]" := nil : list_scope.
-Local Notation "[ a ; .. ; b ]" := (a :: .. (b :: []) ..) : list_scope.
+Local Notation "[ a ; .. ; b ]" := (a :: .. (b :: nil) ..) : list_scope.
 (* Import ListNotations. *) (* in Coq 8.4 *)
 
 Inductive ListOperation : Type :=
@@ -21,9 +22,9 @@ Inductive ListOperation : Type :=
 
 Inductive ListOperationLength : ListOperation -> nat -> nat -> Prop :=
   | LengthEmpty  : ListOperationLength EmptyOp 0 0
-  | LengthRetain : forall o n m, ListOperationLength o n m -> ListOperationLength (RetainOp o) (S n) (S m)
-  | LengthInsert : forall a o n m, ListOperationLength o n m -> ListOperationLength (InsertOp a o) n (S m)
-  | LengthDelete : forall o n m, ListOperationLength o n m -> ListOperationLength (DeleteOp o) (S n) m.
+  | LengthRetain : forall o m n, ListOperationLength o m n -> ListOperationLength (RetainOp o) (S m) (S n)
+  | LengthInsert : forall a o m n, ListOperationLength o m n -> ListOperationLength (InsertOp a o) m (S n)
+  | LengthDelete : forall o m n, ListOperationLength o m n -> ListOperationLength (DeleteOp o) (S m) n.
 
 Hint Constructors ListOperationLength.
 
@@ -48,15 +49,24 @@ Proof.
   intros o. induction o; constructor; assumption.
 Qed.
 
-Lemma operation_length_deterministic : forall o n m n' m',
-  ListOperationLength o n m ->
-  ListOperationLength o n' m' ->
-  n = n' /\ m = m'.
+Lemma operation_length_deterministic : forall o m n m' n',
+  ListOperationLength o m n ->
+  ListOperationLength o m' n' ->
+  m = m' /\ n = n'.
 Proof with auto.
   intros o. induction o; intros n m n' m' L1 L2; inversion L1; inversion L2; subst...
     destruct (IHo _ _ _ _ H0 H4)...
     destruct (IHo _ _ _ _ H3 H8)...
     destruct (IHo _ _ _ _ H0 H4)...
+Qed.
+
+Lemma operation_length_comb : forall o m n,
+  ListOperationLength o m n ->
+  m = start_length o /\ n = end_length o.
+Proof.
+  intros o m n H.
+  assert (ListOperationLength o (start_length o) (end_length o)) as H' by apply operation_length.
+  apply (operation_length_deterministic _ _ _ _ _ H H').
 Qed.
 
 Fixpoint apply (o : ListOperation) (l : list A) : option (list A) :=
@@ -68,9 +78,17 @@ Fixpoint apply (o : ListOperation) (l : list A) : option (list A) :=
   | _,             _       => None
   end.
 
-Theorem apply_length : forall (o : ListOperation) (l : list A) (m : nat),
-  ListOperationLength o (length l) m ->
-  exists l', apply o l = Some l' /\ length l' = m.
+Lemma option_map_None : forall {S T : Type} (f : S -> T) (o : option S),
+  option_map f o = None <-> o = None.
+Proof.
+  intros. split; intros H.
+    destruct o. inversion H. reflexivity.
+    rewrite H. reflexivity.
+Qed.
+
+Lemma apply_length : forall (o : ListOperation) (l : list A) (n : nat),
+  ListOperationLength o (length l) n ->
+  exists l', apply o l = Some l' /\ length l' = n.
 Proof with auto.
   intros o. induction o; intros.
     inversion H. destruct l.
@@ -91,6 +109,18 @@ Proof with auto.
         assumption.
 Qed.
 
+Lemma apply_wrong_length : forall (o : ListOperation) (l : list A),
+  start_length o <> length l ->
+  apply o l = None.
+Proof with auto.
+  intros o. induction o; intros l H; destruct l as [| x xs]...
+    contradiction H...
+    simpl. rewrite option_map_None. apply IHo. intros Eq. apply H. simpl. rewrite Eq. reflexivity.
+    simpl. rewrite option_map_None. apply IHo. assumption.
+    simpl. rewrite option_map_None. apply IHo. assumption.
+    simpl. apply IHo. intros Eq. apply H. simpl. rewrite Eq. reflexivity.
+Qed.
+
 Fixpoint compose (a : ListOperation) : ListOperation -> option ListOperation :=
   fix compose' (b : ListOperation) : option (ListOperation) :=
     match a, b with
@@ -103,6 +133,189 @@ Fixpoint compose (a : ListOperation) : ListOperation -> option ListOperation :=
     | InsertOp _ a', DeleteOp b'   => compose a' b'
     | _,             _             => None
     end.
+
+Lemma compose_length : forall (a : ListOperation) (b : ListOperation) m n o,
+  ListOperationLength a m n ->
+  ListOperationLength b n o ->
+  exists ab, compose a b = Some ab /\ ListOperationLength ab m o.
+Proof with auto.
+  intros a. induction a; intros.
+  (* EmptyOp *)
+    apply operation_length_comb in H; simpl in H; destruct H; subst.
+    generalize dependent o. induction b; intros; try solve [inversion H0].
+    (* EmptyOp *)
+      exists EmptyOp...
+    (* InsertOp *)
+      inversion H0; subst. destruct (IHb _ H4) as [ab' [P Q]].
+      exists (InsertOp a ab'). split... unfold compose. fold (compose EmptyOp). rewrite P...
+  (* RetainOp *)
+    apply operation_length_comb in H; simpl in H; destruct H; subst.
+    generalize dependent o. induction b; intros; try solve [inversion H0].
+    (* RetainOp *)
+      inversion H0; subst. destruct (IHa _ _ _ _ (operation_length a) H2) as [ab' [P Q]].
+      exists (RetainOp ab'). split... unfold compose. fold (compose a). rewrite P...
+    (* InsertOp *)
+      inversion H0; subst. destruct (IHb _ H4) as [ab' [P Q]].
+      exists (InsertOp a0 ab'). split... unfold compose. fold (compose (RetainOp a)). rewrite P...
+    (* DeleteOp *)
+      inversion H0; subst. destruct (IHa _ _ _ _ (operation_length a) H2) as [ab' [P Q]].
+      exists (DeleteOp ab'). split... simpl. rewrite P...
+  (* InsertOp *)
+    rename a into c. rename a0 into a.
+    apply operation_length_comb in H; simpl in H; destruct H; subst.
+    generalize dependent o. induction b; intros; try solve [inversion H0].
+    (* RetainOp *)
+      inversion H0; subst. destruct (IHa _ _ _ _ (operation_length a) H2) as [ab' [P Q]].
+      exists (InsertOp c ab'). split... unfold compose. fold (compose a). rewrite P...
+    (* InsertOp *)
+      inversion H0; subst. destruct (IHb _ H4) as [ab' [P Q]].
+      exists (InsertOp a0 ab'). split... unfold compose. fold (compose (InsertOp c a)). rewrite P...
+    (* DeleteOp *)
+      inversion H0; subst. destruct (IHa _ _ _ _ (operation_length a) H2) as [ab' [P Q]].
+      exists ab'...
+  (* DeleteOp *)
+    inversion H; subst. destruct (IHa _ _ _ _ H2 H0) as [ab' [P Q]].
+    exists (DeleteOp ab'). split... unfold compose. fold compose. destruct b; rewrite P...
+Qed.
+
+Lemma compose_wrong_length : forall a b,
+  end_length a <> start_length b ->
+  compose a b = None.
+Proof with auto.
+  intros a. induction a; intros.
+  (* EmptyOp *)
+    induction b...
+    (* EmptyOp *)
+      contradiction H...
+    (* InsertOp *)
+      unfold compose. fold (compose EmptyOp). rewrite option_map_None. apply IHb...
+  (* RetainOp *)
+    induction b...
+    (* RetainOp *)
+      unfold compose. fold compose. rewrite option_map_None. apply IHa.
+      intros Eq. apply H. simpl. rewrite Eq...
+    (* InsertOp *)
+      unfold compose. fold (compose (RetainOp a)). rewrite option_map_None. apply IHb...
+    (* DeleteOp *)
+      unfold compose. fold compose. rewrite option_map_None. apply IHa.
+      intros Eq. apply H. simpl. rewrite Eq...
+  (* InsertOp *)
+    induction b...
+    (* RetainOp *)
+      unfold compose. fold compose. rewrite option_map_None. apply IHa.
+      intros Eq. apply H. simpl. rewrite Eq...
+    (* InsertOp *)
+      unfold compose. fold (compose (InsertOp a a0)). rewrite option_map_None. apply IHb...
+    (* DeleteOp *)
+      simpl. apply IHa.
+      intros Eq. apply H. simpl. rewrite Eq...
+  (* DeleteOp *)
+    simpl. destruct b; simpl; rewrite option_map_None; apply IHa; assumption.
+Qed.
+
+Lemma compose_EmptyOp_left : forall b,
+  start_length b = 0 ->
+  compose EmptyOp b = Some b.
+Proof with auto.
+  intros b. induction b; intros H; inversion H...
+  (* InsertOp *) unfold compose. fold (compose EmptyOp). rewrite IHb...
+Qed.
+
+Lemma compose_EmptyOp_right : forall a,
+  end_length a = 0 ->
+  compose a EmptyOp = Some a.
+Proof with auto.
+  intros a. induction a; intros H; inversion H...
+  (* DeleteOp *) unfold compose. fold compose. rewrite IHa...
+Qed.
+
+Definition option_join {T} (m : option (option T)) : option T :=
+  match m with
+  | None    => None
+  | Some m' => m'
+  end.
+
+Lemma option_map_compose : forall S T U (f : S -> T) (g : T -> U) (m : option S),
+  option_map g (option_map f m) = option_map (fun x => g (f x)) m.
+Proof with auto.
+  intros. destruct m...
+Qed.
+
+Lemma option_map_join : forall S T U (f : S -> option T) (g : T -> U) (m : option S),
+  option_map g (option_join (option_map f m)) =
+  option_join (option_map (fun x => option_map g (f x)) m).
+Proof with auto.
+  intros. destruct m...
+Qed.
+
+Definition compose_correct : forall a b l,
+  option_join (option_map (apply b) (apply a l)) = option_join (option_map (fun ab => apply ab l) (compose a b)).
+Proof with auto.
+  intros a b l.
+  destruct (eq_nat_dec (end_length a) (start_length b)) as [e | e].
+  (* end_length a = start_length b *)
+    destruct (eq_nat_dec (length l) (start_length a)) as [e0 | e0].
+    (* length l = start_length a *)
+      generalize dependent b. generalize dependent l. induction a; intros.
+      (* EmptyOp *)
+        rewrite compose_EmptyOp_left... destruct l as [| x xs]... inversion e0.
+      (* RetainOp *)
+        destruct l as [| x xs]. inversion e0.
+        induction b; intros; inversion e; inversion e0...
+        (* RetainOp *)
+          unfold compose. fold compose.
+          simpl. do 2 rewrite option_map_compose.
+          simpl. do 2 rewrite <- option_map_join.
+          rewrite IHa...
+        (* InsertOp *)
+          unfold compose. fold (compose (RetainOp a)).
+          replace (apply (InsertOp a0 b)) with (fun x => option_map (fun y => a0 :: y) (apply b x)) by reflexivity.
+          rewrite <- option_map_join. rewrite IHb...
+          rewrite option_map_compose. simpl.
+          rewrite <- option_map_join...
+        (* DeleteOp *)
+          unfold compose. fold compose.
+          simpl. do 2 rewrite option_map_compose.
+          rewrite IHa...
+      (* InsertOp *)
+        rename a into c. rename a0 into a.
+        induction b; intros; inversion e.
+        (* RetainOp *)
+          unfold compose. fold compose.
+          simpl. do 2 rewrite option_map_compose.
+          simpl. do 2 rewrite <- option_map_join.
+          rewrite IHa...
+        (* InsertOp *)
+          unfold compose. fold (compose (InsertOp c a)).
+          replace (apply (InsertOp a0 b)) with (fun x => option_map (fun y => a0 :: y) (apply b x)) by reflexivity.
+          rewrite <- option_map_join. rewrite IHb...
+          rewrite option_map_compose. simpl.
+          rewrite <- option_map_join...
+        (* DeleteOp *)
+          unfold compose. fold compose.
+          simpl. rewrite option_map_compose.
+          rewrite IHa...
+      (* DeleteOp *)
+        destruct l as [| x xs]. inversion e0.
+        simpl. rewrite IHa...
+        destruct b; rewrite option_map_compose; reflexivity.
+  (* length l <> start_length a *)
+    apply not_eq_sym in e0. rewrite (apply_wrong_length a l)...
+    set (La := operation_length a). rewrite e in La.
+    set (Lb := operation_length b).
+    destruct (compose_length _ _ _ _ _ La Lb) as [ab [Eq_ab Lab]].
+    rewrite Eq_ab. simpl. destruct (operation_length_comb _ _ _ Lab) as [H _].
+    symmetry. apply (apply_wrong_length ab l). rewrite <- H...
+    (* end_length a <> start_length b *)
+      rewrite compose_wrong_length...
+      destruct (eq_nat_dec (start_length a) (length l)).
+      (* length l = start_length a *)
+        set (La := operation_length a). rewrite e0 in La.
+        destruct (apply_length _ _ _ La) as [l' [Eq_l' Len_l']]. rewrite Eq_l'.
+        simpl. apply apply_wrong_length. rewrite Len_l'...
+      (* length l <> start_length a *)
+        rewrite apply_wrong_length...
+Qed.
 
 Definition pair_map {A A' B B' : Type} (f : A -> A') (g : B -> B') (p : A * B) : A' * B' :=
   pair (f (fst p)) (g (snd p)).
